Our covariance function is
```math
k(x_i, x_j) = 2r^2\log r - (1+2\log R)r^2 + R^2, \quad \text{where} \ r = ||x_i - x_j||
```
1. The first partial derivative with respect to $x_i$ is calculated as follows:
```math
\frac{\partial k}{\partial x_i} = \frac{\partial k}{\partial r} \frac{\partial r}{\partial x_i} \\ 
```
```math
\begin{align}
\frac{\partial k}{\partial r} &= \frac{\partial}{\partial r} (2r^2\log r - (1+2\log R)r^2 + R^2) \\
 & = 4r \log r + 2r^2.\frac{1}{r} - (1+2\log R)2r + 0 \\
 & = 4r \log r + 2r - 2r - 4r\log R \\
 & = 4r (\log r - \log R)\\
\\
\frac{\partial r}{\partial x_i} &= \frac{x_i - x_j}{r}
\end{align}
```
  
&nbsp; &nbsp; &nbsp;  Now from the chain rule we get:
```math
\begin{align}
\frac{\partial k}{\partial x_i} &= 4r (\log r - \log R) \cdot \frac{x_i - x_j}{r}\\
&= 4 (\log r - \log R) (x_i - x_j)
\end{align}
```


2. The first partial derivative with respect to $x_j$ is calculated as follows:
```math
\frac{\partial k}{\partial x_j} = \frac{\partial k}{\partial r} \frac{\partial r}{\partial x_i} \\ 
```
```math
\begin{align}
\frac{\partial k}{\partial r} &= 4r (\log r - \log R)\\
\frac{\partial r}{\partial x_j} &= \frac{x_j - x_i}{r} \\
 &= -\frac{x_i - x_j}{r}
\end{align}
```
  
&nbsp; &nbsp; &nbsp;  Now from the chain rule we get:
```math
\begin{align}
\frac{\partial k}{\partial x_j} &= 4r (\log r - \log R) \cdot (-\frac{x_i - x_j}{r})\\
&= -4 (\log r - \log R) (x_i - x_j)
\end{align}
```

3. To find the second mixed partial derivative, we need to differentiate $\frac{\partial k}{\partial x_i}$ with respect to $x_j$:   
```math
\begin{align}
\frac{\partial^2}{\partial x_i \partial x_j} k(x_i, x_j) &= \frac{\partial}{\partial x_j} \left( \frac{\partial k}{\partial x_i} \right) \\
 &= \frac{\partial}{\partial x_j} \left( 4 (\log r - \log R) (x_i - x_j) \right) \\
 &= 4 \left[ \frac{\partial}{\partial x_j} (\log r - \log R) \cdot (x_i - x_j) + (\log r - \log R) \cdot \frac{\partial}{\partial x_j} (x_i - x_j) \right] \\
 &= 4 \left[ \frac{\partial}{\partial x_j} (\log r) \cdot (x_i - x_j) + (\log r - \log R) \cdot (-I) \right] \\
 &= 4 \left[ \frac{1}{r} \cdot \frac{\partial r}{\partial x_j} \cdot (x_i - x_j) - (\log r - \log R)I \right] \\
 &= 4 \left[ \frac{1}{r} \left(\frac{x_j-x_i}{r} \right) \cdot (x_i - x_j) - (\log r - \log R) I \right] \\
 &= 4 \left[ -\frac{x_i-x_j}{r^2} \cdot (x_i - x_j) - (\log r - \log R) I \right] \\
 &= -4 \left[\frac{(x_i - x_j)(x_i - x_j)^T}{r^2} + (\log r - \log R) I \right]
\end{align}
```
